examples/single_coin/SingleCoinIAproof.v
@@ -1,5 +1,6 @@
 Require Import CRIS.
 Require Import SingleCoinIPproof SingleCoinPAproof.
+Require Import ProphecyFacts.
 
 Module SingleCoinIA. Section SingleCoinIA.
   Context `{!crisG Γ Σ α β τ _S _I, !concGS, !prophGS, !coinGS}.
@@ -7,10 +8,23 @@ Module SingleCoinIA. Section SingleCoinIA.
 
   Local Notation CoinI := (SingleCoinI.t).
   Local Notation CoinA := (SingleCoinA.t sp).
-  Local Notation ProphA := (ProphecyA.t sp).
 
-  (* Lemma ctxr (md : Mod.t) : refines (CoinA ★ md, emp%I) (CoinI ★ md, emp%I).
+  Lemma ctxr (md : Mod.t) :
+    real_mod md →
+    refines
+      (CoinA ★ md, ProphecyA.initial_cond ∗ SingleCoinA.init_cond)%I
+      (CoinI ★ md, emp%I).
   Proof.
-    etr
-  Qed. *)
+    intros Hreal.
+    etrans; cycle 1.
+    { eapply prophecy_refines with (Pm:=emp%I); eauto.
+      { intros mn; eapply main_adequacy, SingleCoinIP.sim. }
+      { intros mn; eapply main_adequacy, SingleCoinPA.sim. }
+      { intros mn. rewrite /real_mod.
+        mod_tac (s; esplits; ii; edestruct excluded_middle_informative; ss).
+      }
+    }
+    eapply ctxr_refines, ctxr_cond_strengthen; iIntros "[$ $] //".
+  Unshelve. all: apply True.
+  Qed.
 End SingleCoinIA. End SingleCoinIA.
