prophecy/ProphecyFacts.v
@@ -1,4 +1,4 @@
-Require Export CRIS CallFilter ProphecyHeader ProphecyIAproof ProphecyI ProphecyA.
+Require Export CRIS CallFilter ProphecyIAproof.
 
 Lemma CFilter_real_mod `{Σ : GRA} (md : Mod.t) (msk : gset string) :
   real_mod md → real_mod (CFilter.filter msk md).
@@ -7,7 +7,6 @@ Proof.
   intros Hix i x; rewrite lookup_fmap; specialize (Hix i); destruct lookup as [[[? ?]|]|];
     i; clarify; destruct x; ss; clarify.
   { rewrite /CFilter.msk_filter /=; eapply (Hix (Some (e, f))); ss. }
-  eapply (Hix None); auto.
 Qed.
 
 Section prophecy.
@@ -33,41 +32,63 @@ Section prophecy.
   Local Lemma maxlen_union s1 s2 : maxlen (s1 ++ s2) = maxlen s1 `max` maxlen s2.
   Proof. rewrite /maxlen fmap_app list_max_app //. Qed.
 
-  Lemma prophecy_refines (mds mdt : Mod.t) (mdm : string → Mod.t) (Pm Ps : iProp Σ) :
+  Lemma prophecy_refines (mds mdt ctx : Mod.t) (mdm : string → Mod.t) (Pm Ps : iProp Σ) :
     (∀ mn,
       ctx_refines
         (mdm mn ★ ProphecyI.t mn, Pm)
-        (CFilter.filter (exports mn) mdt ★ ProphecyI.t mn, emp%I)) →
+        (CFilter.filter (ProphecyName.exports mn) mdt ★ ProphecyI.t mn, emp%I)) →
     (∀ mn,
       ctx_refines
         (mds, Ps)
         (mdm mn ★ ProphecyA.t mn ∅, emp%I)) →
     (∀ mn, real_mod (mdm mn)) →
-    refines (mds, Pm ∗ ProphecyA.initial_cond ∗ Ps)%I (mdt, emp%I).
+    real_mod ctx →
+    refines (mds ★ ctx, Pm ∗ ProphecyA.initial_cond ∗ Ps)%I (mdt ★ ctx, emp%I).
   Proof.
-    intros Hproph Hreal.
-    set (mn :=
-      maxlen (elements (set_omap id (dom (Mod.fnsems mdt)) : gset string) ++ Mod.scopes mdt)).
+    intros Hproph Hreal ? ?.
+    set (mn := maxlen
+      (elements (set_omap id (dom (Mod.fnsems (mdt ★ ctx))) : gset string) ++
+       (* elements (set_omap id (dom (Mod.fnsems ctx)) : gset string) ++ *)
+       elements (set_omap id (dom (Mod.fnsems (ctx ★ mds))) : gset string) ++
+      Mod.scopes mdt ++ Mod.scopes ctx ++ Mod.scopes mds)).
     etrans; cycle 1.
-    { eapply ctxr_refines, CFilter.intro_filter with (fns := exports (mname_long (S mn))). }
+    { eapply ctxr_refines,
+        CFilter.intro_filter with (fns := ProphecyName.exports (mname_long (S mn))). }
     etrans; cycle 1.
     { eapply CFilter.intro_module with (mc := ProphecyI.t (mname_long (S mn))).
       { econs; [mod_tac|prove_nodup]. }
       { set_solver. }
-      { intros i Hi1 Hi2; rewrite -elem_of_elements in Hi1; eapply elem_of_maxlen in Hi1.
+      { intros i Hi1 Hi2; rewrite -elem_of_elements in Hi1; eapply elem_of_maxlen in Hi1;
         set_unfold; des; subst mn; subst; ss;
-          rewrite mname_long_length maxlen_union in Hi1; lia.
+          rewrite ?mname_long_length ?maxlen_union in Hi1; lia.
       }
       { set_solver+. }
       { set_solver+. }
     }
-    etrans; last eapply ctxr_refines, (Hproph (mname_long (S mn))).
+    rewrite CFilter.filter_app.
     etrans; cycle 1.
-    { eapply ProphIA.adequacy_refines; eauto. }
-    eapply ctxr_refines.
+    { eapply ctxr_refines.
+      ctxr_rotate. ctxr_drop. ctxr_rotate.
+      eapply (Hproph (mname_long (S mn))).
+    }
     etrans; cycle 1.
-    { ctxr_norm; eauto. }
-    eapply ctxr_cond_strengthen; iIntros "[$ [$ $]]".
+    { rewrite Mod.add_comm mod_add_assoc (Mod.add_comm (ProphecyI.t _)) -mod_add_assoc.
+      eapply ProphIA.adequacy_refines; eauto.
+      eapply real_mod_add; eauto using CFilter_real_mod.
+    }
+    etrans; cycle 1.
+    { eapply ctxr_refines. ctxr_rotate. ctxr_drop. ctxr_rotate. eapply Hreal. }
+    etrans; cycle 1.
+    { eapply ctxr_refines. ctxr_drop. eapply CFilter.intro_filter. }
+    erewrite <-!CFilter.filter_app. ctxr_norm.
+    etrans; cycle 1.
+    { eapply CFilter.elim_filter.
+      intros i Hi1 Hi2; rewrite -elem_of_elements in Hi1; eapply elem_of_maxlen in Hi1;
+        set_unfold; des; subst mn; subst; ss;
+          rewrite ?mname_long_length ?maxlen_union in Hi1; lia.
+    }
+
+    rewrite Mod.add_comm.
+    eapply ctxr_refines, ctxr_cond_strengthen; iIntros "[$ [$ $]]".
   Qed.
-    
 End prophecy.
